code/experimental/P256/Hacl.Spec.P256.MontgomeryMultiplication.PointDouble.fst
@@ -14,17 +14,15 @@ open Hacl.Spec.P256.MontgomeryMultiplication
 open Lib.Loops
 open FStar.Mul
 
+#set-options "--z3rlimit 300" 
 let _point_double p =
   let x, y, z = p in 
-  if z = 0 then (x, y, z)
-  else begin 
   let s = (4 * x * y * y) % prime in 
   let m = ((-3) * z * z * z * z + 3 * x * x) % prime in 
-  let x3 = (m *m - 2 * s) % prime in 
+  let x3 = (m * m - 2 * s) % prime in 
   let y3 = (m * (s - x3) - 8 * y * y * y * y) % prime in 
-  let z3 = (2 * y * z) % prime in (x3, y3, z3)
-  end
-
+  let z3 = (2 * y * z) % prime in 
+  (x3, y3, z3)
 
 
 val computeS: px: felem_seq{felem_seq_as_nat px < prime} -> py: felem_seq{felem_seq_as_nat py < prime} -> 
@@ -40,6 +38,7 @@ let computeS px py =
   let pyD = fromDomain_ (felem_seq_as_nat py) in 
   let a = montgomery_multiplication_seq py py in 
   let b = montgomery_multiplication_seq px a in 
+    lemma_mod_mul_distr_r pxD (pyD * pyD) prime;  
   let s = mm_byFour_seq b in 
   
   assert_by_tactic (pxD * (pyD * pyD) == pxD * pyD * pyD) canon;
@@ -48,9 +47,8 @@ let computeS px py =
   lemma_mod_mul_distr_r 4 (pxD * pyD * pyD) prime
 
 val computeM: px: felem_seq{felem_seq_as_nat px < prime} -> pz: felem_seq{felem_seq_as_nat pz < prime} -> 
-  Lemma ((
-   let pxD = fromDomain_ (felem_seq_as_nat px) in let pzD = fromDomain_(felem_seq_as_nat pz) in 
-   let m = felem_add_seq (mm_byMinusThree_seq(mm_quatre_seq pz)) (mm_byThree_seq(montgomery_multiplication_seq px px)) in  
+  Lemma ((let pxD = fromDomain_ (felem_seq_as_nat px) in let pzD = fromDomain_(felem_seq_as_nat pz) in 
+  let m = felem_add_seq (mm_byMinusThree_seq(mm_quatre_seq pz)) (mm_byThree_seq(montgomery_multiplication_seq px px)) in  
   felem_seq_as_nat m = toDomain_ ((((-3) * pzD * pzD * pzD * pzD + 3 * pxD * pxD) % prime)))) 
 
 let computeM px pz = 
@@ -93,7 +91,6 @@ let computeZ3 py pz =
 
 
 #reset-options "--z3rlimit 100" 
-
 val lemma_xToSpecification: pxD: nat -> pyD: nat -> pzD: nat -> 
   s: felem_seq{felem_seq_as_nat s = toDomain_ (4 * pxD * pyD * pyD % prime)} -> 
   m: felem_seq{felem_seq_as_nat m = toDomain_ ((((-3) * pzD * pzD * pzD * pzD + 3 * pxD * pxD)) % prime)} -> 
@@ -102,6 +99,7 @@ val lemma_xToSpecification: pxD: nat -> pyD: nat -> pzD: nat ->
   Lemma ((let (xN, yN, zN) = _point_double (pxD, pyD, pzD) in felem_seq_as_nat x3 = toDomain_ (xN)))
 
 let lemma_xToSpecification pxD pyD pzD s m x3  = ()
+
 
 val lemma_yToSpecification: pxD: nat -> pyD: nat -> pzD: nat ->
   s: felem_seq{felem_seq_as_nat s = toDomain_ (4 * pxD * pyD * pyD % prime)} -> 
@@ -115,32 +113,35 @@ val lemma_yToSpecification: pxD: nat -> pyD: nat -> pzD: nat ->
 
 let lemma_yToSpecification pxD pyD pzD s m x3 y3 = ()
 
+
 val lemma_zToSpecification: pxD: nat ->  pyD: nat -> pzD: nat -> 
   z3: felem_seq{felem_seq_as_nat z3 = toDomain_(2 * pyD * pzD % prime)} -> 
   Lemma (let (xN, yN, zN) = _point_double (pxD, pyD, pzD) in felem_seq_as_nat z3 = toDomain_ (zN))
 
 let lemma_zToSpecification pxD pyD pzD z3 = ()
 
-let isPointAtInfinitySeq p = 
-    let a0 = Lib.Sequence.index p 8 in 
-    let a1 = Lib.Sequence.index p 9 in 
-    let a2 = Lib.Sequence.index p 10 in 
-    let a3 = Lib.Sequence.index p 11 in 
-    let a_tuple = (a0, a1, a2, a3) in 
-    let r = isZero_tuple_b a_tuple in 
-    
 
-    let z = Lib.Sequence.sub p 8 4 in 
-    let z_seq = felem_seq_as_nat z in 
-    assert_norm (modp_inv2 (pow2 256) > 0);
-    assert_norm (modp_inv2 (pow2 256) % prime <> 0);
-    lemma_multiplication_not_mod_prime z_seq (modp_inv2 (pow2 256));
-    r
-
+noextract
+val copy_point_seq: p: point_seq -> Tot (r: point_seq{p == r})
 
 #reset-options "--z3rlimit 100" 
-
 let copy_point_seq p = p
+
+
+noextract
+val point_double_compute_s_m_seq:  
+  p: point_seq
+    {let x = Lib.Sequence.sub p 0 4 in let y = Lib.Sequence.sub p 4 4 in let z = Lib.Sequence.sub p 8 4 in felem_seq_as_nat x < prime /\ felem_seq_as_nat y < prime /\ felem_seq_as_nat z < prime} -> 
+  Tot (r: tuple2 felem_seq felem_seq{let s, m = r in 
+      let px = Lib.Sequence.sub p 0 4 in 
+      let py = Lib.Sequence.sub p 4 4 in 
+      let pz = Lib.Sequence.sub p 8 4 in   
+      let pxD = fromDomain_ (felem_seq_as_nat px) in 
+      let pyD = fromDomain_ (felem_seq_as_nat py) in 
+      let pzD = fromDomain_ (felem_seq_as_nat pz) in 
+      felem_seq_as_nat s == toDomain_(4 * pxD * pyD * pyD % prime) /\
+      felem_seq_as_nat m == toDomain_ ((((-3) * pzD * pzD * pzD * pzD + 3 * pxD * pxD) % prime))
+  })
 
 let point_double_compute_s_m_seq p = 
   let px = Lib.Sequence.sub p 0 4 in 
@@ -162,13 +163,26 @@ let point_double_compute_s_m_seq p =
   (s, m)
 
 
+noextract
+val point_double_compute_x3_seq: s: felem_seq {felem_seq_as_nat s < prime} -> 
+  m: felem_seq{felem_seq_as_nat m < prime} -> 
+  Tot (x3: felem_seq {
+    let mD = fromDomain_ (felem_seq_as_nat m) in let sD = fromDomain_ (felem_seq_as_nat s) in 
+    felem_seq_as_nat x3 < prime /\ felem_seq_as_nat x3 = toDomain_ (((mD * mD - 2 * sD) % prime))})
+
 let point_double_compute_x3_seq s m = 
   let twoS = mm_byTwo_seq s in 
   let mm = montgomery_multiplication_seq m m in 
   let x3 = felem_sub_seq mm twoS in 
   lemma_minus_distr ((fromDomain_ (felem_seq_as_nat m)) * (fromDomain_ (felem_seq_as_nat m))) (2 * (fromDomain_ (felem_seq_as_nat s))); 
   x3
- 
+
+
+noextract
+val point_double_compute_y3_seq: p_y: felem_seq{felem_seq_as_nat p_y < prime} -> x3: felem_seq {felem_seq_as_nat x3 < prime}->  s: felem_seq{felem_seq_as_nat s < prime} -> m: felem_seq{felem_seq_as_nat m < prime} -> Tot (y3: felem_seq {
+   let mD = fromDomain_ (felem_seq_as_nat m) in let sD = fromDomain_ (felem_seq_as_nat s) in let x3D = fromDomain_ (felem_seq_as_nat x3) in let pyD = fromDomain_ (felem_seq_as_nat p_y) in
+felem_seq_as_nat y3 < prime /\ felem_seq_as_nat y3 = toDomain_ (((mD * (sD - x3D) - (8 * pyD * pyD * pyD * pyD))% prime))})
+
 let point_double_compute_y3_seq py x3 s m = 
     let open FStar.Tactics in 
     let open FStar.Tactics.Canon in 
@@ -190,7 +204,20 @@ let point_double_compute_y3_seq py x3 s m =
     lemma_mod_mul_distr_r 8 (pyD * pyD * pyD * pyD) prime;
     lemma_minus_distr (mD * (sD - x3D)) (8 * pyD * pyD * pyD * pyD);
     y3
-  
+
+
+noextract
+val point_double_seq: p: point_seq{let x = Lib.Sequence.sub p 0 4 in let y = Lib.Sequence.sub p 4 4 in let z = Lib.Sequence.sub p 8 4 in 
+  felem_seq_as_nat x < prime /\ felem_seq_as_nat y < prime /\ felem_seq_as_nat z < prime} -> 
+  Tot (r: point_seq  {
+    let x3 = Lib.Sequence.sub r 0 4 in let y3 = Lib.Sequence.sub r 4 4 in let z3 = Lib.Sequence.sub r 8 4 in 
+    let x = Lib.Sequence.sub p 0 4 in let y = Lib.Sequence.sub p 4 4 in let z = Lib.Sequence.sub p 8 4 in 
+    
+    let xD = fromDomain_ (felem_seq_as_nat x) in let yD = fromDomain_ (felem_seq_as_nat y) in let zD = fromDomain_(felem_seq_as_nat z) in 
+ 
+    let (xN, yN, zN) = _point_double (xD, yD, zD) in 
+    felem_seq_as_nat x3 = toDomain_ (xN) /\ felem_seq_as_nat y3 = toDomain_ (yN) /\ felem_seq_as_nat z3 = toDomain_ (zN) /\ felem_seq_as_nat x3 < prime /\ felem_seq_as_nat y3 < prime /\ felem_seq_as_nat z3 < prime
+    }) 
 
 let point_double_seq p =
   let open FStar.Tactics in 
@@ -199,16 +226,6 @@ let point_double_seq p =
   let px = Lib.Sequence.sub p 0 4 in 
   let py = Lib.Sequence.sub p 4 4 in 
   let pz = Lib.Sequence.sub p 8 4 in 
-
-  let p_infinity = isPointAtInfinitySeq p in 
-  if p_infinity then 
-    begin
-      lemmaFromDomainToDomain (felem_seq_as_nat px);
-      lemmaFromDomainToDomain (felem_seq_as_nat py);
-      lemmaFromDomainToDomain (felem_seq_as_nat pz);
-      copy_point_seq p 
-    end
-  else begin
 
   let (s, m) = point_double_compute_s_m_seq p in 
   let x3 = point_double_compute_x3_seq s m in 
@@ -219,10 +236,8 @@ let point_double_seq p =
   let r = concat (concat x3 y3) z3 in
   
   computeZ3 py pz;
-  
   lemma_xToSpecification (fromDomain_ (felem_seq_as_nat px)) (fromDomain_ (felem_seq_as_nat py)) (fromDomain_ (felem_seq_as_nat pz)) s m x3;
   lemma_yToSpecification (fromDomain_ (felem_seq_as_nat px)) (fromDomain_ (felem_seq_as_nat py)) (fromDomain_ (felem_seq_as_nat pz)) s m x3 y3;
   lemma_zToSpecification (fromDomain_ (felem_seq_as_nat px)) (fromDomain_ (felem_seq_as_nat py)) (fromDomain_ (felem_seq_as_nat pz)) z3;
   r
-  end
-
+ 
